semantics/proofs/fpSemPropsScript.sml
@@ -8,38 +8,38 @@ open terminationTheory;
 val _ = new_theory "fpSemProps";
 
 Theorem fp_opts_mono[local]:
-  ! (s1 s2 s3:'a state) n m.
-    (! x. s1.fp_opts (n + x) = s2.fp_opts x) /\
-    (! x. s2.fp_opts (m + x) = s3.fp_opts x) ==>
-    ? k. ! x. s1.fp_opts (k + x) = s3.fp_opts x
+  ! (fps1 fps2 fps3:fp_state) n m.
+    (! x. fps1.opts (n + x) = fps2.opts x) /\
+    (! x. fps2.opts (m + x) = fps3.opts x) ==>
+    ! x. fps1.opts ((m+n) + x) = fps3.opts x
 Proof
-  rpt strip_tac \\ qexists_tac `n+m`
-  \\ qpat_x_assum `! x. _ _ = s3.fp_opts _` (qspec_then `x` (fn thm => fs[GSYM thm]))
-  \\ qpat_x_assum `! x. _ _ = s2.fp_opts _` (qspec_then `m + x` (fn thm => fs[GSYM thm]))
+  rpt strip_tac \\ fs[]
+  \\ qpat_x_assum `! x. _ _ = fps3.opts _` (qspec_then `x` (fn thm => fs[GSYM thm]))
+  \\ qpat_x_assum `! x. _ _ = fps2.opts _` (qspec_then `m + x` (fn thm => fs[GSYM thm]))
 QED
 
 Theorem fp_opts_add_1[local]:
-  ! (s1 s2:'a state) n m.
-    (! x. s1.fp_opts (n + x) = s2.fp_opts x) ==>
-    ? k. ! x. s1.fp_opts (k + x) = s2.fp_opts (x + 1)
+  ! (fps1 fps2:fp_state) n m.
+    (! x. fps1.opts (n + x) = fps2.opts x) ==>
+    ! x. fps1.opts ((n + 1) + x) = fps2.opts (x + 1)
 Proof
-  rpt strip_tac
-  \\ qexists_tac `n+1` \\ fs[]
+  rpt strip_tac \\ fs[]
 QED
 
 Theorem evaluate_fp_opts_inv:
-  (! (s1:'a state) env e s2 r.
-    evaluate s1 env e = (s2, r) ==>
-    (! x. s1.fp_opts (x + (s2.fp_choices - s1.fp_choices)) = s2.fp_opts x) /\
-    s1.fp_rws = s2.fp_rws /\
-    s1.fp_choices <= s2.fp_choices /\
-    (?c. 0 <= c /\ c = s2.fp_choices - s1.fp_choices)) /\
-  (! (s1:'a state) env v pes errv s2 r.
-    evaluate_match s1 env v pes errv = (s2, r) ==>
-    (! x. s1.fp_opts (x + (s2.fp_choices - s1.fp_choices)) = s2.fp_opts x) /\
-    s1.fp_rws = s2.fp_rws /\
-    s1.fp_choices <= s2.fp_choices /\
-    (?c. 0 <= c /\ c = s2.fp_choices - s1.fp_choices))
+  (! (s1:'a state) env (fps1:fp_state) e s2 fps2 r.
+    evaluate s1 env fps1 e = (s2, fps2, r) ==>
+    (! x. fps1.opts (x + (fps2.choices - fps1.choices)) = fps2.opts x) /\
+    fps1.rws = fps2.rws /\
+    fps1.choices <= fps2.choices) /\
+    (* (?c. 0 <= c /\ c = s2.fp_choices - s1.fp_choices)) /\ *)
+  (! (s1:'a state) env (fps1:fp_state) v pes errv s2 fps2 r.
+    evaluate_match s1 env fps1 v pes errv = (s2, fps2, r) ==>
+    (! x. fps1.opts (x + (fps2.choices - fps1.choices)) = fps2.opts x) /\
+    fps1.rws = fps2.rws /\
+    fps1.choices <= fps2.choices)
+ (* /\
+    (?c. 0 <= c /\ c = s2.fp_choices - s1.fp_choices)) *)
 Proof
   ho_match_mp_tac evaluate_ind \\ rw[]
   \\ rfs[evaluate_def] \\ rveq
@@ -51,29 +51,29 @@ Proof
   \\ imp_res_tac fp_opts_mono
   \\ imp_res_tac fp_opts_add_1
   \\ TRY (asm_exists_tac \\ fs[])
-  \\ rpt (qpat_x_assum `! x. _ = _.fp_opts x`
+  \\ rpt (qpat_x_assum `! x. _ = _.opts x`
             ( fn thm => once_rewrite_tac [GSYM thm])
           \\ fs[])
 QED
 
-(* Write this in terms of +, not -, st2.fp_choices < k + st1.fp_choices *)
 local
   val eval_goal =
-    ``\ st1 env xs.
-      ! st2 r k h.
-        evaluate st1 env xs = (st2, r) /\
-        st2.fp_choices - st1.fp_choices < k /\
-        (! m. m < k ==> h m = st1.fp_opts m) ==>
+    ``\ st1 env fps1 xs.
+      ! st2 fps2 r k h.
+        evaluate st1 env fps1 xs = (st2, fps2, r) /\
+        (* analogous to fps2.choices - fps1.choices < k but easier to use *)
+        fps2.choices < k + fps1.choices /\
+        (! m. m < k ==> h m = fps1.opts m) ==>
           ? hN.
-            evaluate (st1 with fp_opts := h) env xs = (st2 with fp_opts := hN, r)``;
+            evaluate st1 env (fps1 with opts := h) xs = (st2, fps2 with opts := hN, r)``;
   val eval_match_goal =
-    `` \ st1 env v pl err_v.
-        ! st2 r k h.
-          evaluate_match st1 env v pl err_v = (st2, r) /\
-          st2.fp_choices - st1.fp_choices < k /\
-          (! m. m < k ==> h m = st1.fp_opts m) ==>
+    `` \ st1 env fps1 v pl err_v.
+        ! st2 fps2 r k h.
+          evaluate_match st1 env fps1 v pl err_v = (st2, fps2, r) /\
+          fps2.choices < k + fps1.choices /\
+          (! m. m < k ==> h m = fps1.opts m) ==>
             ? hN.
-              evaluate_match (st1 with fp_opts := h) env v pl err_v = (st2 with fp_opts := hN, r)``;
+              evaluate_match st1 env (fps1 with opts := h) v pl err_v = (st2, fps2 with opts := hN, r)``;
   val indThm = terminationTheory.evaluate_ind
     |> ISPEC eval_goal |> SPEC eval_match_goal;
   val eval_fp_opt_invs = evaluate_fp_opts_inv;
@@ -81,72 +81,71 @@ local
   val evalmatch_fp_opt_inv = hd (tl (CONJ_LIST 2 evaluate_fp_opts_inv));
   val solve_simple =
     rpt strip_tac \\ rveq \\ first_x_assum drule \\ rpt (disch_then drule)
-    \\ disch_then assume_tac \\ fs[state_component_equality];
+    \\ disch_then assume_tac \\ fs[fp_state_component_equality];
     (* \\ rename1 `evaluate (st with fp_opts := _) _ _ = (st2, _)`
         ORELSE rename1 `evaluate_match (st with fp_opts := _) _ _ _ _ = (st2, _)`
     \\ qexists_tac `st2` \\ fs[];*)
   val solve_complex =
     rpt strip_tac \\ rveq
     \\ imp_res_tac eval_fp_opt_invs
-    \\ (rename [`evaluate stA env [e1] = (stB, Rval r)`,
-            `evaluate stB _ _ = (stC, _)`]
+    \\ (rename [`evaluate _ env fpA [e1] = (_, fpB, Rval r)`,
+            `evaluate _ _ fpB _ = (_, fpC , _)`]
       ORELSE
-        rename [`evaluate stA env (REVERSE es) = (stB, Rval r)`,
-            `evaluate (dec_clock stB) _ _ = (stC, _)`]
+        rename [`evaluate _ env fpA (REVERSE es) = (_, fpB, Rval r)`,
+            `evaluate (dec_clock _) _ fpB _ = (_, fpC, _)`]
       ORELSE
-      rename [`evaluate stA env _ = (stB, _)`,
-            `evaluate_match stB _ _ _ _ = (stC, _)`])
+      rename [`evaluate _ env fpA _ = (_, fpB, _)`,
+            `evaluate_match _ _ fpB _ _ _ = (_ , fpC, _)`])
     \\ fs[dec_clock_def]
-    \\ `stB.fp_choices < k + stA.fp_choices` by (fs[])
+    \\ `fpB.choices < k + fpA.choices` by (fs[])
     \\ last_x_assum (qspecl_then [`k`, `h`] drule)
     \\ rpt (disch_then drule) \\ disch_then assume_tac \\ fs[]
-    \\ `! x. x < (k - (stB.fp_choices - stA.fp_choices)) ==> hN x = stB.fp_opts x`
+    \\ `! x. x < (k - (fpB.choices - fpA.choices)) ==> hN x = fpB.opts x`
       by (first_x_assum (mp_then Any assume_tac eval_fp_opt_inv) \\ fs[]
           \\ rveq \\ rpt strip_tac
           \\ qpat_x_assum `! x. h _ = hN _` (fn thm => fs[GSYM thm]))
-    \\ `stC.fp_choices < (k -(stB.fp_choices - stA.fp_choices)) + stB.fp_choices` by fs[]
-    \\ `0 < k - (stB.fp_choices - stA.fp_choices)` by  fs[]
-    \\ res_tac \\ fs[state_component_equality];
+    \\ `fpC.choices < (k - (fpB.choices - fpA.choices)) + fpB.choices` by fs[]
+    \\ `0 < k - (fpB.choices - fpA.choices)` by  fs[]
+    \\ res_tac \\ fs[fp_state_component_equality];
 in
 Theorem evaluate_fp_opt_add_bind:
-  (! (st1:'a state) env xs.
-    ^eval_goal st1 env xs) /\
-  (! (st1:'a state) env v pl err_v.
-    ^eval_match_goal st1 env v pl err_v)
+  (! (st1:'a state) env fps1 xs.
+    ^eval_goal st1 env fps1 xs) /\
+  (! (st1:'a state) env fps1 v pl err_v.
+    ^eval_match_goal st1 env fps1 v pl err_v)
 Proof
   match_mp_tac indThm
   \\ rpt strip_tac \\ fs[evaluate_def]
-  \\ rpt strip_tac \\ fs[state_component_equality] \\ rveq
-  \\ qpat_x_assum `_ = (_,_)` mp_tac
+  \\ rpt strip_tac \\ fs[fp_state_component_equality] \\ rveq
+  \\ qpat_x_assum `_ = (_,_,_)` mp_tac
   >- (
-    ntac 2 (reverse TOP_CASE_TAC \\ fs[]) >- solve_simple
-    \\ ntac 2 (TOP_CASE_TAC \\ fs[])
+    ntac 3 (reverse TOP_CASE_TAC \\ fs[]) >- solve_simple
+    \\ ntac 3 (TOP_CASE_TAC \\ fs[])
     \\ solve_complex)
   >- (
-    ntac 2 (reverse TOP_CASE_TAC \\ fs[]) >- solve_simple
+    ntac 3 (reverse TOP_CASE_TAC \\ fs[]) >- solve_simple
     \\ rpt strip_tac \\ rveq
-    \\ res_tac \\ fs[state_component_equality])
+    \\ res_tac \\ fs[fp_state_component_equality])
   >- (
-    ntac 2 (TOP_CASE_TAC \\ fs[]) >- solve_simple
+    ntac 3 (TOP_CASE_TAC \\ fs[]) >- solve_simple
     \\ reverse TOP_CASE_TAC \\ fs[]
     >- solve_simple
     \\ solve_complex)
   >- (
     reverse TOP_CASE_TAC \\ fs[]
-    >- solve_simple
-    \\ ntac 2 (reverse TOP_CASE_TAC \\ fs[])
+    >- (rpt strip_tac \\ fs[fp_state_component_equality])
+    \\ ntac 3 (reverse TOP_CASE_TAC \\ fs[])
     >- solve_simple
     \\ reverse TOP_CASE_TAC \\ fs[]
     >- solve_simple
     \\ rpt strip_tac \\ rveq
     \\ imp_res_tac eval_fp_opt_invs
     \\ res_tac \\ fs[]
-    \\ fs[state_component_equality])
+    \\ fs[fp_state_component_equality])
   >- (
-    reverse TOP_CASE_TAC \\ fs[]
-    \\ solve_simple)
+    reverse TOP_CASE_TAC \\ fs[fp_state_component_equality])
   >- (
-    ntac 2 (reverse TOP_CASE_TAC \\ fs[])
+    ntac 3 (reverse TOP_CASE_TAC \\ fs[])
     >- solve_simple
     \\ TOP_CASE_TAC \\ fs[]
     >- (TOP_CASE_TAC \\ fs[]
@@ -159,64 +158,72 @@ Proof
     \\ ntac 3 (reverse TOP_CASE_TAC \\ fs[])
     \\ rpt strip_tac \\ fs[shift_fp_opts_def]
     \\ imp_res_tac eval_fp_opt_invs
-    \\ rename [`evaluate st1 env (REVERSE _) = (st2, _)`]
-    \\ rveq \\ fs[state_component_equality]
-    \\ `st2.fp_choices < k + st1.fp_choices` by (fs[dec_clock_def])
+    \\ rename [`evaluate _ env fps1 (REVERSE _) = (_, fps2, _)`]
+    \\ rveq \\ fs[fp_state_component_equality]
+    \\ `fps2.choices < k + fps1.choices` by (fs[dec_clock_def])
     \\ last_x_assum (qspecl_then [`k`, `h`] drule)
-    \\ rpt (disch_then drule) \\ disch_then assume_tac \\ fs[state_component_equality]
-    \\ `hN 0 = st2.fp_opts 0` suffices_by fs[]
+    \\ rpt (disch_then drule) \\ disch_then assume_tac \\ fs[fp_state_component_equality]
+    \\ `hN 0 = fps2.opts 0` suffices_by fs[]
     \\ first_x_assum (mp_then Any assume_tac eval_fp_opt_inv) \\ fs[]
     \\ rveq \\ rpt strip_tac
     \\ qpat_x_assum `! x. h _ = hN _` (fn thm => fs[GSYM thm])
-    \\ qpat_x_assum `!x. st1.fp_opts _ = st2.fp_opts _` (fn thm => fs[GSYM thm]))
-  >- (ntac 2 (reverse TOP_CASE_TAC \\ fs[]) >- solve_simple
+    \\ qpat_x_assum `!x. fps1.opts _ = fps2.opts _` (fn thm => fs[GSYM thm]))
+  >- (
+      ntac 3 (reverse TOP_CASE_TAC \\ fs[]) >- solve_simple
       \\ TOP_CASE_TAC \\ fs[] >- solve_simple
       \\ reverse TOP_CASE_TAC \\ fs[] >- solve_simple
       \\ solve_complex)
-  >- (ntac 2 (reverse TOP_CASE_TAC \\ fs[]) >- solve_simple
+  >- (
+      ntac 3 (reverse TOP_CASE_TAC \\ fs[]) >- solve_simple
       \\ TOP_CASE_TAC \\ fs[] >- solve_simple
       \\ solve_complex)
-  >- (ntac 2 (reverse TOP_CASE_TAC \\ fs[]) >- solve_simple
+  >- (
+      ntac 3 (reverse TOP_CASE_TAC \\ fs[]) >- solve_simple
       \\ solve_complex)
-  >- (ntac 2 (reverse TOP_CASE_TAC \\ fs[]) >- solve_simple
+  >- (
+      ntac 3 (reverse TOP_CASE_TAC \\ fs[]) >- solve_simple
       \\ solve_complex)
-  >- (reverse TOP_CASE_TAC \\ fs[] >- solve_simple
-      \\ rpt strip_tac \\ rveq \\ res_tac \\ fs[state_component_equality])
-  >- (rpt strip_tac \\ last_x_assum match_mp_tac
+  >- (
+      reverse TOP_CASE_TAC \\ fs[fp_state_component_equality]
+      \\ rpt strip_tac \\ rveq \\ res_tac \\ fs[fp_state_component_equality])
+  >- (
+      rpt strip_tac \\ last_x_assum match_mp_tac
       \\ fs[] \\ asm_exists_tac \\ fs[])
-  >- (rpt strip_tac \\ last_x_assum match_mp_tac
+  >- (
+      rpt strip_tac \\ last_x_assum match_mp_tac
       \\ fs[] \\ asm_exists_tac \\ fs[])
-  >- (ntac 2 (reverse TOP_CASE_TAC \\ fs[])
-      >- (rpt strip_tac \\ rveq
+  >- (
+      ntac 3 (reverse TOP_CASE_TAC \\ fs[])
+      >- (
+          rpt strip_tac \\ rveq
           \\ first_x_assum (qspecl_then [`k`, `h`] assume_tac)
           \\ fs[]
           \\ res_tac \\ fs[]
-          \\ qexists_tac `hN` \\ fs[state_component_equality])
-      \\ rpt strip_tac \\ rveq \\ fs[state_component_equality]
-      \\ res_tac \\ fs[state_component_equality])
-  >- (reverse TOP_CASE_TAC \\ fs[] >- solve_simple
-      \\ TOP_CASE_TAC \\ fs[] \\ solve_simple)
+          \\ qexists_tac `hN` \\ fs[fp_state_component_equality])
+      \\ rpt strip_tac \\ rveq \\ fs[fp_state_component_equality]
+      \\ res_tac \\ fs[fp_state_component_equality])
+  >- (reverse TOP_CASE_TAC \\ fs[fp_state_component_equality]
+      \\ TOP_CASE_TAC \\ fs[fp_state_component_equality] \\ solve_simple)
 QED
 
   local
     val eval_fp_opt_add_bind = hd (CONJ_LIST 2 (SIMP_RULE std_ss [] evaluate_fp_opt_add_bind));
   in
 Theorem evaluate_fp_opt_add_bind_preserving:
-  ! (st1 st2:'ffi state) env xs r k h.
-    evaluate st1 env xs = (st2, r) /\
-    st2.fp_choices - st1.fp_choices < k /\
-    (! m. m < k ==> h m = st1.fp_opts m) ==>
+  ! (st1 st2:'a state) env fps1 fps2 xs r k h.
+    evaluate st1 env fps1 xs = (st2, fps2, r) /\
+    fps2.choices < k + fps1.choices /\
+    (! m. m < k ==> h m = fps1.opts m) ==>
     ? hN.
-      evaluate (st1 with fp_opts := h) env xs =
-        (st2 with fp_opts := hN, r) /\
-      (! m. m < (k - (st2.fp_choices - st1.fp_choices)) ==> hN m = st2.fp_opts m) /\
-      (hN (k - (st2.fp_choices - st1.fp_choices)) = h k)
+      evaluate st1 env (fps1 with opts := h) xs =
+        (st2, fps2 with opts := hN, r) /\
+      (! m. m < (k - (fps2.choices - fps1.choices)) ==> hN m = fps2.opts m) /\
+      (hN (k - (fps2.choices - fps1.choices)) = h k)
 Proof
   rpt strip_tac
   \\ first_assum (mp_then Any assume_tac eval_fp_opt_add_bind)
-  \\ pop_assum (fn asm => first_assum (mp_then Any assume_tac asm)) \\ fs[]
-  \\ res_tac
-  \\ ntac 2 (pop_assum kall_tac) \\ fs[state_component_equality]
+  \\ pop_assum (fn asm => last_assum (mp_then Any assume_tac asm)) \\ fs[]
+  \\ res_tac \\ fs[fp_state_component_equality]
   \\ first_assum (mp_then Any assume_tac eval_fp_opt_inv)
   \\ last_assum (mp_then Any assume_tac eval_fp_opt_inv)
   \\ fs[] \\ conj_tac \\ rpt strip_tac
@@ -226,10 +233,10 @@ QED
 end;
 
 Theorem fpOp_determ:
-  ! op refs refsN (ffi1 ffi1':'a ffi_state) (ffi2:'b ffi_state) r vl.
+  ! op refs refsN (ffi1 ffi2:'a ffi_state) (ffi3:'b ffi_state) r vl.
     isFpOp op /\
-    do_app (refs, ffi1) op vl = SOME ((refsN, ffi1'), r) ==>
-    do_app (refs, ffi2) op vl = SOME ((refsN, ffi2), r)
+    do_app (refs, ffi1) op vl = SOME ((refsN, ffi2), r) ==>
+    do_app (refs, ffi3) op vl = SOME ((refsN, ffi3), r)
 Proof
   rpt strip_tac \\ Cases_on `op` \\ fs[astTheory.isFpOp_def]
   \\ rpt (qpat_x_assum `do_app _ _ _ = _` mp_tac)
