semantics/terminationScript.sml
@@ -165,7 +165,7 @@ val _ = register "rwAllBoolTree" rwAllBoolTree_def rwAllBoolTree_ind;
 
 val (nsMap_def, nsMap_ind) =
   tprove_no_defn ((nsMap_def, nsMap_ind),
-  wf_rel_tac `measure (\(_, env). namespace_size (\x. 1) (\x. 1) (\x. 1) env)`
+  wf_rel_tac `measure (\ (_, env). namespace_size (\x. 1) (\x. 1) (\x. 1) env)`
   >> Induct_on `m`
   >> rw [namespace_size_def]
   >> rw [namespace_size_def]
@@ -317,14 +317,14 @@ QED
 
 val fix_clock_IMP = Q.prove(
   `fix_clock s x = (s1,res) ==> s1.clock <= s.clock`,
-  Cases_on `x` \\ fs [fix_clock_def] \\ rw [] \\ fs []);
+  PairCases_on `x` \\ fs [fix_clock_def] \\ rw [] \\ fs []);
 
 val (evaluate_def, evaluate_ind) =
   tprove_no_defn ((evaluateTheory.evaluate_def,evaluateTheory.evaluate_ind),
   wf_rel_tac`inv_image ($< LEX $<)
     (λx. case x of
-         | INL(s,_,es) => (s.clock,exps_size es)
-         | INR(s,_,_,pes,_) => (s.clock,pes_size pes))` >>
+         | INL(s,_,_, es) => (s.clock,exps_size es)
+         | INR(s,_,_,_, pes,_) => (s.clock,pes_size pes))` >>
   rw[size_abbrevs,exp_size_def,
   dec_clock_def,LESS_OR_EQ,
   do_if_def,do_log_def] >>
@@ -332,8 +332,8 @@ val (evaluate_def, evaluate_ind) =
   simp[SIMP_RULE(srw_ss())[]exps_size_thm,MAP_REVERSE,SUM_REVERSE]);
 
 Theorem evaluate_clock:
-   (∀(s1:'ffi state) env e r s2. evaluate s1 env e = (s2,r) ⇒ s2.clock ≤ s1.clock) ∧
-   (∀(s1:'ffi state) env v p v' r s2. evaluate_match s1 env v p v' = (s2,r) ⇒ s2.clock ≤ s1.clock)
+   (∀(s1:'ffi state) env fps e r s2. evaluate s1 env fps e = (s2,r) ⇒ s2.clock ≤ s1.clock) ∧
+   (∀(s1:'ffi state) env fps v p v' r fps2 s2. evaluate_match s1 env fps v p v' = (s2,r) ⇒ s2.clock ≤ s1.clock)
 Proof
   ho_match_mp_tac evaluate_ind >> rw[evaluate_def] >>
   every_case_tac >> fs[] >> rw[] >> rfs[] >>
@@ -341,18 +341,24 @@ Proof
   imp_res_tac fix_clock_IMP >> fs[]
 QED
 
-Theorem fix_clock_evaluate:
-   fix_clock s1 (evaluate s1 env e) = evaluate s1 env e
+Theorem fix_clock_alt:
+  fix_clock s1 (s2, r) = (s2 with clock := if s2.clock <= s1.clock then s2.clock else s1.clock, r)
 Proof
-  Cases_on `evaluate s1 env e` \\ fs [fix_clock_def]
+  PairCases_on `r` \\ fs[fix_clock_def]
+QED
+
+Theorem fix_clock_evaluate:
+   fix_clock s1 (evaluate s1 env fps e) = evaluate s1 env fps e
+Proof
+  Cases_on `evaluate s1 env fps e` \\ fs [fix_clock_alt]
   \\ imp_res_tac evaluate_clock
   \\ fs [MIN_DEF,state_component_equality]
 QED
 
 Theorem fix_clock_evaluate_fp_canOpt:
-   fix_clock s1 (evaluate (s1 with fp_canOpt := T) env e) = evaluate (s1 with fp_canOpt := T) env e
+   fix_clock s1 (evaluate s1 env (fps with canOpt := T) e) = evaluate s1 env (fps with canOpt := T) e
 Proof
-  Cases_on `evaluate (s1 with fp_canOpt := T) env e` \\ fs [fix_clock_def]
+  Cases_on `evaluate s1 env (fps with canOpt := T) e` \\ fs [fix_clock_alt]
   \\ imp_res_tac evaluate_clock
   \\ fs [MIN_DEF,state_component_equality]
 QED
@@ -377,7 +383,7 @@ QED
 
 val (evaluate_decs_def,evaluate_decs_ind) =
   tprove_no_defn ((evaluate_decs_def,evaluate_decs_ind),
-  wf_rel_tac `measure (list_size dec_size o SND o SND)` >>
+  wf_rel_tac `measure (list_size dec_size o SND o SND o SND)` >>
   rw [dec1_size_eq]);
 
 val _ = register "evaluate_decs" evaluate_decs_def evaluate_decs_ind
